Prove safety for mutex

src/examples/mutex.v
@@ -12,6 +12,7 @@ Example: (spinlock) Mutex
 
 This example is a liveness proof for the following simple C program. It encodes the program as a hand-written state machine, with states referring to labeled points.
 
+```
 type Mutex = bool;
 const UNLOCKED = false;
 const LOCKED = true;
@@ -26,6 +27,7 @@ void unlock(Mutex *m) {
   *m = UNLOCKED;
   // s2
 }
+```
 
 What we reason about is two threads running lock(m); unlock(m) (assuming m starts out allocated).
 
@@ -33,7 +35,7 @@ What we reason about is two threads running lock(m); unlock(m) (assuming m start
 
 Module spec.
 
-  Inductive pc := s0 | s1 | s2.
+  Inductive pc := pc0 | pc1 | pc2.
   Inductive Tid := tid0 | tid1.
 
   #[global]
@@ -51,23 +53,89 @@ Module spec.
   Instance _eta : Settable _ := settable! mkState <lock; pcs>.
 
   Definition cas_fail (t0: Tid): action state :=
-    λ s s', (s.(pcs) t0 = s0 ∧ s.(lock) = true)
+    λ s s', (s.(pcs) t0 = pc0 ∧ s.(lock) = true)
             ∧ s' = s.
 
   Definition cas_succ (t0: Tid): action state :=
-    λ s s', s.(pcs) t0 = s0 ∧ s.(lock) = false
+    λ s s', s.(pcs) t0 = pc0 ∧ s.(lock) = false
             ∧ s' = s <|lock := true|>
-                     <|pcs ::= <[ t0 := s1 ]> |>.
+                     <|pcs ::= <[ t0 := pc1 ]> |>.
 
   Definition unlock (t0: Tid): action state :=
-    λ s s', s.(pcs) t0 = s1
+    λ s s', s.(pcs) t0 = pc1
             ∧ s' = s <|lock := false|>
-                     <|pcs ::= <[ t0 := s2 ]> |>.
+                     <|pcs ::= <[ t0 := pc2 ]> |>.
 
   Definition step (t0: Tid): action state :=
       λ s s', cas_fail t0 s s' ∨ cas_succ t0 s s' ∨ unlock t0 s s'.
 
+  Definition init: state → Prop :=
+    λ s, s = {| lock := false; pcs := λ _, pc0; |}.
+
   Definition next : action state :=
     λ s s', step tid0 s s' ∨ step tid1 s s' ∨ s' = s.
 
+  (* safety is mutual exclusion *)
+  Definition safe: state → Prop :=
+    λ s, ¬ (s.(pcs) tid0 = pc1 ∧ s.(pcs) tid1 = pc1).
+
+  Definition fair: predicate state :=
+    weak_fairness (step tid0) ∧ weak_fairness (step tid1).
+
+  (* liveness means both threads terminate *)
+  Definition terminated: state → Prop :=
+    λ s, s.(pcs) tid0 = pc2 ∧ s.(pcs) tid1 = pc2.
+
 End spec.
+
+Import spec.
+
+Section example.
+
+Implicit Types (s: state) (t: Tid).
+
+Hint Unfold init next step safe fair terminated : stm.
+
+Ltac stm_simp :=
+  autounfold with stm;
+  intros; (intuition (repeat deex; subst; trivial));
+  rewrite ?enabled_eq;
+  repeat deex;
+  (* TODO: why does this infinite loop? *)
+  do 10 (try match goal with
+        | s: state |- _ => destruct s; cbn in *
+        | H: @eq pc _ _ |- _ => inversion H; subst; clear H
+        | H: @eq state (mkState _ _) (mkState _ _) |- _ =>
+            inversion H; subst; clear H
+        end);
+  cbn in *.
+
+Ltac stm :=
+  stm_simp;
+  try solve [ intuition (repeat deex; eauto) ].
+
+Definition exclusion_inv: state → Prop :=
+  λ s, (s.(pcs) tid0 = pc1 → s.(lock) ∧ s.(pcs) tid1 ≠ pc1) ∧
+       (s.(pcs) tid1 = pc1 → s.(lock) ∧ s.(pcs) tid0 ≠ pc1).
+
+Hint Unfold exclusion_inv : stm.
+
+Hint Unfold cas_fail cas_succ unlock : stm.
+
+Lemma exclusion_inv_ok :
+  ⌜init⌝ ∧ □⟨next⟩ ⊢ □⌜exclusion_inv⌝.
+Proof.
+  apply init_invariant.
+  - stm.
+  - stm.
+Qed.
+
+Theorem safety :
+  ⌜init⌝ ∧ □⟨next⟩ ⊢ □⌜safe⌝.
+Proof.
+  rewrite -> exclusion_inv_ok.
+  apply always_impl_proper.
+  unseal; stm.
+Qed.
+
+End example.
